src/ByteStringHeap.v
@@ -19,109 +19,110 @@ Import FMapExt.
 
 Open Scope N_scope.
 
-Record PS (heapType : Type) := makePS {
-  psHeap   : heapType;
+Record PS := makePS {
   psBuffer : Ptr Word;
   psBufLen : Size;
   psOffset : Size;
   psLength : Size
 }.
 
-Definition PSH := PS (Rep HeapSpec).
-
-Definition simply_widen_region (r : PSH) : PSH :=
-  {| psHeap   := psHeap r
-   ; psBuffer := psBuffer r
+Definition simply_widen_region (r : PS) : PS :=
+  {| psBuffer := psBuffer r
    ; psBufLen := psBufLen r
    ; psOffset := psOffset r - 1
    ; psLength := psLength r + 1 |}.
 
-Program Definition make_room_by_shifting_up (r : PSH) (n : N | 0 < n) :
+Definition make_room_by_shifting_up
+        (h : Rep HeapSpec) (r : PS) (n : N | 0 < n) :
   (* We could maybe be smarter by shifting the block so it sits mid-way within
      the buffer. *)
-  Comp PSH :=
-  res <- memcpy (psHeap r) (psBuffer r) (psBuffer r + n) (psLength r);
-  ret {| psHeap   := fst res
-       ; psBuffer := psBuffer r
-       ; psBufLen := psBufLen r
-       ; psOffset := 0
-       ; psLength := psLength r + n |}.
+  Comp (Rep HeapSpec * PS) :=
+  res <- memcpy h (psBuffer r) (psBuffer r + ` n) (psLength r);
+  ret (fst res,
+       {| psBuffer := psBuffer r
+        ; psBufLen := psBufLen r
+        ; psOffset := 0
+        ; psLength := psLength r + ` n |}).
 
-Program Definition make_room_by_growing_buffer (r : PSH) (n : N | 0 < n) :
-  Comp PSH :=
+Program Definition make_room_by_growing_buffer
+        (h : Rep HeapSpec) (r : PS) (n : N | 0 < n) :
+  Comp (Rep HeapSpec * PS) :=
   (* We can make a trade-off here by allocating extra bytes in anticipation of
      future calls to [buffer_cons]. *)
-  `(h, a) <- alloc (psHeap r) (psLength r + n);
+  `(h, a) <- alloc h (psLength r + n);
   `(h, _) <- memcpy h (psBuffer r) (a + n) (psLength r);
   `(h, _) <- free h (psBuffer r);
-  ret {| psHeap   := h
-       ; psBuffer := a
-       ; psBufLen := psLength r + n
-       ; psOffset := 0
-       ; psLength := psLength r + n |}.
+  ret (h, {| psBuffer := a
+           ; psBufLen := psLength r + n
+           ; psOffset := 0
+           ; psLength := psLength r + n |}).
 Obligation 1. nomega. Defined.
 
-Program Definition allocate_buffer (r : Rep HeapSpec) (len : N | 0 < len) :
-  Comp PSH :=
-  `(h, a) <- alloc r len;
-  ret {| psHeap   := h
-       ; psBuffer := a
-       ; psBufLen := len
-       ; psOffset := 0
-       ; psLength := len |}.
+Program Definition allocate_buffer (h : Rep HeapSpec) (len : N | 0 < len) :
+  Comp (Rep HeapSpec * PS) :=
+  `(h, a) <- alloc h len;
+  ret (h, {| psBuffer := a
+           ; psBufLen := len
+           ; psOffset := 0
+           ; psLength := len |}).
 
-Definition poke_at_offset (r : PSH) (d : Word) : Comp PSH :=
-  res <- poke (psHeap r) (psBuffer r + psOffset r) d;
-  ret {| psHeap   := fst res
-       ; psBuffer := psBuffer r
-       ; psBufLen := psBufLen r
-       ; psOffset := psOffset r
-       ; psLength := psLength r |}.
+Definition poke_at_offset (h : Rep HeapSpec) (r : PS) (d : Word) :
+  Comp (Rep HeapSpec * PS) :=
+  res <- poke h (psBuffer r + psOffset r) d;
+  ret (fst res,
+       {| psBuffer := psBuffer r
+        ; psBufLen := psBufLen r
+        ; psOffset := psOffset r
+        ; psLength := psLength r |}).
 
 (* This defines how much a buffer is grown by when more space is needed to
    [cons] on a new element. *)
 Definition alloc_quantum := 1.
 Arguments alloc_quantum /.
 
-Program Definition buffer_cons (r : PSH) (d : Word) : Comp PSH :=
-  ps <- If 0 <? psOffset r
-        Then ret (simply_widen_region r)
-        Else
-        If psLength r + alloc_quantum <=? psBufLen r
-        Then make_room_by_shifting_up r alloc_quantum
-        Else
-        If 0 <? psBufLen r
-        Then make_room_by_growing_buffer r alloc_quantum
-        Else allocate_buffer (psHeap r) alloc_quantum;
-  poke_at_offset ps d.
+Program Definition buffer_cons (h : Rep HeapSpec) (r : PS) (d : Word) :
+  Comp (Rep HeapSpec * PS) :=
+  `(h, ps) <-
+    If 0 <? psOffset r
+    Then ret (h, simply_widen_region r)
+    Else
+    If psLength r + alloc_quantum <=? psBufLen r
+    Then make_room_by_shifting_up h r alloc_quantum
+    Else
+    If 0 <? psBufLen r
+    Then make_room_by_growing_buffer h r alloc_quantum
+    Else allocate_buffer h alloc_quantum;
+  poke_at_offset h ps d.
 Obligation 1. nomega. Defined.
 Obligation 2. nomega. Defined.
 Obligation 3. nomega. Defined.
 
-Definition buffer_uncons (r : PSH) : Comp (PSH * option Word) :=
+Definition buffer_uncons (h : Rep HeapSpec) (r : PS) :
+  Comp ((Rep HeapSpec * PS) * option Word) :=
   If 0 <? psLength r
   Then (
-    w <- peek (psHeap r) (psBuffer r + psOffset r);
-    ret ({| psHeap   := psHeap r
-          ; psBuffer := psBuffer r
-          ; psBufLen := psBufLen r
-          ; psOffset := if psLength r =? 1
-                        then 0
-                        else psOffset r + 1
-          ; psLength := psLength r - 1 |}, Some (snd w)))
-  Else ret (r, None).
+    w <- peek h (psBuffer r + psOffset r);
+    ret (h, {| psBuffer := psBuffer r
+             ; psBufLen := psBufLen r
+             ; psOffset := if psLength r =? 1
+                           then 0
+                           else psOffset r + 1
+             ; psLength := psLength r - 1 |}, Some (snd w)))
+  Else ret ((h, r), None).
 
-Definition ByteString_list_AbsR (or : Rep ByteStringSpec) (nr : PSH) :=
-  length or = N.to_nat (psLength nr) /\
-  IF psBufLen nr = 0
-  then psOffset nr = 0 /\ psLength nr = 0
-  else fits (psBuffer nr) (psBufLen nr)
-            (psBuffer nr + psOffset nr) (psLength nr) /\
-       M.MapsTo (psBuffer nr) (psBufLen nr) (resvs (psHeap nr)) /\
-       (forall i, i < psLength nr
+Definition ByteString_list_AbsR
+           (or : Rep ByteStringSpec) (nr : Rep HeapSpec * PS) :=
+  let ps := snd nr in
+  length or = N.to_nat (psLength ps) /\
+  IF psBufLen ps = 0
+  then psOffset ps = 0 /\ psLength ps = 0
+  else fits (psBuffer ps) (psBufLen ps)
+            (psBuffer ps + psOffset ps) (psLength ps) /\
+       M.MapsTo (psBuffer ps) (psBufLen ps) (resvs (fst nr)) /\
+       (forall i, i < psLength ps
           -> forall x, nth (N.to_nat i) or x = x
-          -> forall n, psBuffer nr + psOffset nr + i = n
-          -> M.MapsTo n x (bytes (psHeap nr))).
+          -> forall n, psBuffer ps + psOffset ps + i = n
+          -> M.MapsTo n x (bytes (fst nr))).
 
 Ltac destruct_AbsR H :=
   let H1 := fresh "H1" in
@@ -177,10 +178,10 @@ Proof. destruct b; trivial. Qed.
 
 Lemma buffer_cons_sound : forall r_o r_n,
   ByteString_list_AbsR r_o r_n
-    -> forall x r_n', buffer_cons r_n x ↝ r_n'
+    -> forall x r_n', buffer_cons (fst r_n) (snd r_n) x ↝ r_n'
     -> ByteString_list_AbsR (x :: r_o) r_n'.
 Proof.
-  unfold buffer_cons; intros ? ? AbsR ???.
+  unfold buffer_cons, Bind2; intros ? ? AbsR ???.
   computes_to_inv.
   if_computes_to_inv; subst.
     prepare_AbsR AbsR.
@@ -201,19 +202,18 @@ Proof.
     apply copy_bytes_mapsto.
     rewrite If_Then_Else_MapsTo.
     apply H4 with (i:=i); try nomega.
-    assert (psOffset r_n = 0) as HA by nomega.
+    assert (psOffset (snd r_n) = 0) as HA by nomega.
     rewrite HA, <- H6, !N.add_0_r in *; clear HA H6 n.
-    setoid_replace (x1 + N.succ i - (x1 + 1) + psBuffer r_n)
-      with (psBuffer r_n + i) by nomega.
-    destruct (within_bool _ _ _) eqn:Heqe2; simpl; trivial.
-    nomega.
+    setoid_replace (x1 + N.succ i - (x1 + 1) + psBuffer (snd r_n))
+      with (psBuffer (snd r_n) + i) by nomega.
+    destruct (within_bool _ _ _) eqn:Heqe2; simpl; trivial; nomega.
   prepare_AbsR AbsR.
   reduce_peano i; nomega.
 Qed.
 
 Lemma buffer_uncons_sound : forall r_o r_n a,
   ByteString_list_AbsR r_o r_n
-    -> buffer_uncons r_n ↝ a
+    -> buffer_uncons (fst r_n) (snd r_n) ↝ a
     -> ByteString_list_AbsR (match r_o with
                              | [] => r_o
                              | _ :: xs => xs
@@ -222,7 +222,7 @@ Proof.
   unfold buffer_uncons; intros.
   apply refine_computes_to in H0.
   apply refine_If_Then_Else_bool in H0.
-  destruct (0 <? psLength r_n) eqn:Heqe.
+  destruct (0 <? psLength (snd r_n)) eqn:Heqe.
     revert H0.
     autorewrite with monad laws; simpl; intros.
     apply computes_to_refine in H0.
@@ -232,7 +232,7 @@ Proof.
     destruct r_o; simpl in *;
     try nomega; right;
     split; try nomega; split;
-    destruct (@psLength HeapState r_n =? 1) eqn:Heqe2;
+    destruct (psLength (snd r_n) =? 1) eqn:Heqe2;
     try nomega;
     try (eexists; split; [exact H4|]; nomega).
     split; trivial; intros.
@@ -253,7 +253,7 @@ Qed.
 
 Lemma buffer_uncons_impl : forall r_o r_n a,
   ByteString_list_AbsR r_o r_n
-    -> buffer_uncons r_n ↝ a
+    -> buffer_uncons (fst r_n) (snd r_n) ↝ a
     -> snd a = match r_o with
                | [] => None
                | x :: _ => Some x
@@ -262,7 +262,7 @@ Proof.
   unfold buffer_uncons; intros.
   apply refine_computes_to in H0.
   apply refine_If_Then_Else_bool in H0.
-  destruct (0 <? psLength r_n) eqn:Heqe.
+  destruct (0 <? psLength (snd r_n)) eqn:Heqe.
     revert H0.
     autorewrite with monad laws; simpl; intros.
     apply computes_to_refine in H0.
@@ -271,8 +271,8 @@ Proof.
     destruct r_o; simpl in *; try nomega.
     f_equal; tsubst.
     apply H0.
-    replace (@psBuffer HeapState r_n + @psOffset HeapState r_n)
-       with (@psBuffer HeapState r_n + @psOffset HeapState r_n + 0) by nomega.
+    replace (psBuffer (snd r_n) + psOffset (snd r_n))
+       with (psBuffer (snd r_n) + psOffset (snd r_n) + 0) by nomega.
     eapply H4; eauto; nomega.
   apply computes_to_refine in H0.
   apply Return_inv in H0.
@@ -294,11 +294,11 @@ Proof.
 
   {
     simplify with monad laws.
-    refine pick val {| psHeap   := heap
-                     ; psBuffer := 0
-                     ; psBufLen := 0
-                     ; psOffset := 0
-                     ; psLength := 0 |}.
+    refine pick val (heap,
+                     {| psBuffer := 0
+                      ; psBufLen := 0
+                      ; psOffset := 0
+                      ; psLength := 0 |}).
       finish honing.
     firstorder.
   }
@@ -306,7 +306,7 @@ Proof.
   {
     simplify with monad laws.
     etransitivity.
-      eapply (refine_skip2 (dummy:=buffer_cons r_n d)).
+      eapply (refine_skip2 (dummy:=buffer_cons (fst r_n) (snd r_n) d)).
     etransitivity.
       apply refine_under_bind; intros; simpl.
       refine pick val a.
@@ -320,7 +320,7 @@ Proof.
   {
     simplify with monad laws.
     etransitivity.
-      eapply (refine_skip2 (dummy:=buffer_uncons r_n)).
+      eapply (refine_skip2 (dummy:=buffer_uncons (fst r_n) (snd r_n))).
     etransitivity.
       apply refine_under_bind; intros; simpl.
       pose proof H1.
